WIP porting fundamental to lty causing anomaly

theories/Dot/lr/typeExtractionSem.v
@@ -14,13 +14,11 @@ Section typing_type_member_defs.
      Not sure that's still true if we change dm_to_type,
     but quite possibly yes.. *)
     (* use interp_extractedTy? *)
-  Definition leadsto_envD_equiv s σ (φ : envD Σ) : iProp Σ :=
+  (* Definition leadsto_envD_equiv s σ (φ : envD Σ) : iProp Σ :=
     (∃ (φ' : envD Σ),
       ⌜φ ≡ (λ ρ, φ' (∞ σ.|[ρ]))⌝ ∧ s ↝ φ')%I.
   Arguments leadsto_envD_equiv /.
   Notation "s ↝[  σ  ] φ" := (leadsto_envD_equiv s σ φ) (at level 20).
-
-  Import stamp_transfer.
 
   Lemma extraction_to_leadsto_envD_equiv T g s σ n: T ~[ n ] (g, (s, σ)) →
     wellMappedφ ⟦ g ⟧g -∗ s ↝[ σ ] ty_interp T.
@@ -28,6 +26,18 @@ Section typing_type_member_defs.
     move => [T'] [Hl] [<- [_ /is_stamped_nclosed_ty HclT]].
     iIntros "Hm". iExists (ty_interp T'). iSplitR.
     - iIntros "!%" (ρ v). exact: interp_subst_commute.
+    - iApply (wellMappedφ_apply with "Hm"). by rewrite lookup_fmap Hl.
+  Qed. *)
+  Import stamp_transfer.
+  Import persistent_ty_interp_lemmas.
+
+  Lemma extraction_to_leadsto_envD_equiv T g s σ n: T ~[ n ] (g, (s, σ)) →
+    wellMappedφ ⟦ g ⟧g -∗ s ↝[ σ ] pty_interp T.
+  Proof.
+    move => [T'] [Hl] [<- [_ /is_stamped_nclosed_ty HclT]].
+    iIntros "Hm". iExists (vopen (pty_interp T' vnil)). iSplitR.
+    - iIntros "!%" (args ρ v). rewrite interp_subst_commute //.
+      by dependent destruction args.
     - iApply (wellMappedφ_apply with "Hm"). by rewrite lookup_fmap Hl.
   Qed.
 
@@ -43,20 +53,12 @@ Section typing_type_member_defs.
   Lemma D_Typ_Abs Γ T L U s σ l:
     Γ ⊨ TLater T, 0 <: TLater U, 0 -∗
     Γ ⊨ TLater L, 0 <: TLater T, 0 -∗
-    s ↝[ σ ] ⟦ T ⟧ -∗
+    s ↝[ σ ] p⟦ T ⟧ -∗
     Γ ⊨ { l := dtysem σ s } : TTMem l L U.
-  Proof.
-    iIntros "#HTU #HLT #Hs /= !>" (ρ Hpid) "#Hg".
-    iDestruct "Hs" as (φ Hγφ) "Hγ"; iSplit => //=.
-    iExists (φ _); iSplit. by iApply (dm_to_type_intro with "Hγ").
-    iModIntro; repeat iSplit; iIntros (v) "#HL";
-      rewrite later_intuitionistically.
-    - iIntros "!>". iApply Hγφ. by iApply "HLT".
-    - iApply "HTU" => //. by iApply Hγφ.
-  Qed.
+  Proof. apply sD_Typ_Abs. Qed.
 
   Lemma D_Typ Γ T s σ l:
-    s ↝[ σ ] ⟦ T ⟧ -∗
+    s ↝[ σ ] p⟦ T ⟧ -∗
     Γ ⊨ { l := dtysem σ s } : TTMem l T T.
-  Proof. iIntros "#Hs"; iApply D_Typ_Abs => //; iApply Sub_Refl. Qed.
+  Proof. apply sD_Typ. Qed.
 End typing_type_member_defs.
