theories/Dot/misc_unused/dot_lty.v
@@ -526,6 +526,27 @@ Section defs.
   Qed.
   Context {Γ : ctx}.
 
+  Lemma lift_olty_eq {i} {τ1 τ2 : oltyO Σ i} {args ρ v} :
+    τ1 ≡ τ2 → τ1 args ρ v ≡ τ2 args ρ v.
+  Proof. intros H. apply H. Qed.
+
+  Lemma Sub_Mu_A T i: Γ ⊨ TMu (shift T), i <: T, i.
+  Proof.
+    rewrite /istpi.
+    cbn [pinterp pty_interp].
+    rewrite {1}(pty_interp_subst T (ren (+1))).
+    apply sSub_Mu_A.
+
+    (* iIntros "!>" (vs v) "**".
+    by rewrite /= (lift_olty_eq (pty_interp_subst _ _)). *)
+  Qed.
+
+  Lemma Sub_Mu_B T i: Γ ⊨ T, i <: TMu (shift T), i.
+  Proof.
+    iIntros "!>" (vs v) "**".
+    by rewrite /= (lift_olty_eq (pty_interp_subst _ _)).
+  Qed.
+
   Lemma TMu_I T v: Γ ⊨ tv v : T.|[v/] -∗ Γ ⊨ tv v : TMu T.
   Proof. by rewrite /ietp -sTMu_I pty_interp_subst. Qed.
 
